experiment/Experiment.Steel.Repr.ST_to_SF.Base.fst
@@ -1,0 +1,151 @@
+module Experiment.Steel.Repr.ST_to_SF.Base
+
+module T   = FStar.Tactics
+
+open FStar.Classical.Sugar
+open FStar.Calc
+
+
+#push-options "--fuel 2 --z3rlimit 30"
+let rec repr_SF_of_ST_req
+      (#a : Type u#a) (#pre : ST.pre_t u#b) (#post : ST.post_t u#a u#b a)
+      (t : ST.prog_tree a pre post)
+      (sl0 : Fl.flist pre)
+  : Lemma (ensures ST.tree_req t sl0 <==> tree_req (repr_SF_of_ST t sl0)) (decreases t)
+  = ST.match_prog_tree t
+    (fun a pre post t -> (sl0 : Fl.flist pre) ->
+       squash (ST.tree_req t sl0 <==> tree_req (repr_SF_of_ST t sl0)))
+    (fun (*ST.Tequiv*) pre post0 p -> fun sl0 -> ())
+    begin fun (*ST.Tframe*) a pre post frame f -> fun sl0 ->
+      let (sl0', sl_frame) = Fl.splitAt_ty pre frame sl0 in
+      repr_SF_of_ST_req f sl0'
+    end
+    (fun (*ST.Tspec*) a pre post req ens -> fun sl0 -> ())
+    (fun (*ST.Tret*) a x post -> fun sl0 -> ())
+    begin fun (*ST.Tbind*) a b pre itm post f g -> fun sl0 ->
+      calc (<==>) {
+        ST.tree_req (ST.Tbind a b pre itm post f g) sl0;
+      == { _ by T.(trefl ()) }
+        ST.tree_req f sl0 /\
+        (forall (x : a) (sl1 : Fl.flist (itm x)) .
+          ST.tree_ens f sl0 x sl1 ==> ST.tree_req (g x) sl1);
+      <==> { repr_SF_of_ST_req f sl0;
+           introduce forall (x : a) (sl1 : Fl.flist (itm x)) .
+               (ST.tree_ens f sl0 x sl1 <==> tree_ens (repr_SF_of_ST f sl0) x sl1) /\
+               (ST.tree_req (g x) sl1 <==> tree_req (repr_SF_of_ST (g x) sl1))
+             with (repr_SF_of_ST_ens f sl0 x sl1; repr_SF_of_ST_req (g x) sl1) }
+        tree_req (repr_SF_of_ST f sl0) /\
+        (forall (x : a) (sl1 : Fl.flist (itm x)) .
+          tree_ens (repr_SF_of_ST f sl0) x sl1 ==> tree_req (repr_SF_of_ST (g x) sl1));
+      == { _ by T.(trefl ()) }
+        tree_req (repr_SF_of_ST (ST.Tbind a b pre itm post f g) sl0);
+      }
+    end
+    begin fun (*ST.TbindP*) a b pre post wp f g -> fun sl0 ->
+      introduce forall (x : a) .
+          ST.tree_req (g x) sl0 <==> tree_req (repr_SF_of_ST (g x) sl0)
+        with repr_SF_of_ST_req (g x) sl0;
+      FStar.Monotonic.Pure.elim_pure_wp_monotonicity wp
+    end sl0
+
+and repr_SF_of_ST_ens
+      (#a : Type u#a) (#pre : ST.pre_t u#b) (#post : ST.post_t u#a u#b a)
+      (t : ST.prog_tree a pre post)
+      (sl0 : Fl.flist pre) (res : a) (sl1 : Fl.flist (post res))
+  : Lemma (ensures ST.tree_ens t sl0 res sl1 <==> tree_ens (repr_SF_of_ST t sl0) res sl1) (decreases t)
+  = ST.match_prog_tree t
+    (fun a pre post t -> (sl0 : Fl.flist pre) -> (res : a) -> (sl1 : Fl.flist (post res)) ->
+       squash (ST.tree_ens t sl0 res sl1 <==> tree_ens (repr_SF_of_ST t sl0) res sl1))
+    (fun (*ST.Tequiv*) pre post0 p -> fun sl0 res sl1 -> ())
+    begin fun (*ST.Tframe*) a pre post frame f -> fun sl0 x sl1 ->
+      let sl0', frame0 = Fl.splitAt_ty pre      frame sl0 in
+      let sl1', frame1 = Fl.splitAt_ty (post x) frame sl1 in
+      calc (<==>) {
+        ST.tree_ens (ST.Tframe a pre post frame f) sl0 x sl1;
+      <==> { repr_SF_of_ST_ens f sl0' x sl1' }
+        frame1 == frame0 /\ tree_ens (repr_SF_of_ST f sl0') x sl1';
+      };
+      calc (<==>) {
+        tree_ens (repr_SF_of_ST (ST.Tframe a pre post frame f) sl0) x sl1;
+      <==> { }
+        exists (sl1'_0 : post_v post x) .
+          tree_ens (repr_SF_of_ST f sl0') x sl1'_0 /\ sl1 == Fl.append sl1'_0 frame0;
+      <==> { introduce forall (sl1'_0 : post_v post x) .
+               sl1 == Fl.append sl1'_0 frame0 <==>
+               sl1'_0 == sl1' /\ frame1 == frame0
+             with (Fl.append_splitAt_ty (post x) frame sl1'_0 frame0;
+                   Fl.splitAt_ty_append (post x) frame sl1) }
+        tree_ens (repr_SF_of_ST f sl0') x sl1' /\ frame1 == frame0;
+      }
+    end
+    (fun (*ST.Tspec*) a pre post req ens -> fun sl0 res sl1 -> ())
+    (fun (*ST.Tret*) a x post -> fun sl0 res sl1 -> ())
+    begin fun (*ST.Tbind*) a b pre itm post f g -> fun sl0 y sl2 ->
+      calc (<==>) {
+        ST.tree_ens (ST.Tbind a b pre itm post f g) sl0 y sl2;
+      == { _ by T.(trefl ()) }
+        exists (x : a) (sl1 : post_v itm x) .
+          ST.tree_ens f sl0 x sl1 /\ ST.tree_ens (g x) sl1 y sl2;
+      <==> { introduce forall (x : a) (sl1 : post_v itm x) .
+               (ST.tree_ens f sl0 x sl1 /\ ST.tree_ens (g x) sl1 y sl2) <==>
+               (tree_ens (repr_SF_of_ST f sl0) x sl1 /\ tree_ens (repr_SF_of_ST (g x) sl1) y sl2)
+             with (repr_SF_of_ST_ens f sl0 x sl1; repr_SF_of_ST_ens (g x) sl1 y sl2) }
+        exists (x : a) (sl1 : post_v itm x) .
+          tree_ens (repr_SF_of_ST f sl0) x sl1 /\ tree_ens (repr_SF_of_ST (g x) sl1) y sl2;
+      == { _ by T.(trefl ()) }
+        tree_ens (repr_SF_of_ST (ST.Tbind a b pre itm post f g) sl0) y sl2;
+      }
+    end
+    begin fun (*ST.TbindP*) a b pre post wp f g -> fun sl0 y sl1 ->
+      calc (<==>) {
+        ST.tree_ens (ST.TbindP a b pre post wp f g) sl0 y sl1;
+      == { _ by T.(trefl ()) }
+        exists (x : a) . as_ensures wp x /\ ST.tree_ens (g x) sl0 y sl1;
+      <==> { introduce forall (x : a) .
+               ST.tree_ens (g x) sl0 y sl1 <==> tree_ens (repr_SF_of_ST (g x) sl0) y sl1
+             with repr_SF_of_ST_ens (g x) sl0 y sl1 }
+        exists (x : a) . as_ensures wp x /\ tree_ens (repr_SF_of_ST (g x) sl0) y sl1;
+      == { _ by T.(trefl ()) }
+        tree_ens (repr_SF_of_ST (ST.TbindP a b pre post wp f g) sl0) y sl1;
+      }
+    end sl0 res sl1
+#pop-options
+
+#push-options "--fuel 2 --z3rlimit 20"
+let rec repr_SF_of_ST_shape
+      (#a : Type u#a) (#pre : ST.pre_t u#b) (#post : ST.post_t u#a u#b a)
+      (t : ST.prog_tree a pre post)
+      (#post_n : nat) (s : ST.shape_tree (L.length pre) post_n)
+      (sl0 : Fl.flist pre)
+  : Lemma (requires ST.prog_has_shape t s)
+          (ensures  prog_has_shape (repr_SF_of_ST t sl0) (shape_SF_of_ST s))
+          (decreases t)
+  = ST.match_prog_tree t
+    (fun a pre post t -> (#post_n : nat) -> (s : ST.shape_tree (L.length pre) post_n) ->
+       squash (ST.prog_has_shape t s) ->
+       (sl0 : Fl.flist pre) -> 
+       squash (prog_has_shape (repr_SF_of_ST t sl0) (shape_SF_of_ST s)))
+    (fun (*ST.Tequiv*) pre post0 p -> fun s _ sl0 -> ())
+    begin fun (*ST.Tframe*) a pre post frame f -> fun s _ sl0 ->
+      let ST.Sframe _ post_n _ s_f = s            in
+      let sl0' = (Fl.splitAt_ty pre frame sl0)._1 in
+      repr_SF_of_ST_shape f s_f sl0'
+    end
+    (fun (*ST.Tspec*) a pre post req ens -> fun s _ sl0 -> ())
+    (fun (*ST.Tret*) a x post -> fun s _ sl0 -> ())
+    begin fun (*ST.Tbind*) a b pre itm post f g -> fun s _ sl0 ->
+      let ST.Sbind _ itm_n post_n s_f s_g = s in
+      repr_SF_of_ST_shape f s_f sl0;
+      introduce forall (x : a) (sl1 : Fl.flist (itm x)) .
+           prog_has_shape (repr_SF_of_ST (g x) sl1) (shape_SF_of_ST s_g)
+        with repr_SF_of_ST_shape (g x) s_g sl1
+    end
+    begin fun (*ST.TbindP*) a b pre post wp f g -> fun s _ sl0 ->
+      let ST.SbindP _ post_n s_g = s in
+      let lem_g (x : a)
+        : Lemma (prog_has_shape (repr_SF_of_ST (g x) sl0) (shape_SF_of_ST s_g))
+                [SMTPat (g x)]
+        = repr_SF_of_ST_shape (g x) s_g sl0
+      in ()
+    end s () sl0
+#pop-options
