experiment/Experiment.Steel.Repr.ST_to_SF.Base.fsti
@@ -1,0 +1,74 @@
+module Experiment.Steel.Repr.ST_to_SF.Base
+
+module U   = Learn.Util
+module L   = FStar.List.Pure
+module Ll  = Learn.List
+module Fl  = Learn.FList
+module Dl  = Learn.DList
+module ST  = Experiment.Steel.Repr.ST
+
+open Experiment.Steel.Repr.ST
+open Experiment.Steel.Repr.SF
+
+
+#set-options "--fuel 1 --ifuel 1"
+
+let rec repr_SF_of_ST
+      (#a : Type u#a) (#pre : ST.pre_t u#b) (#post : ST.post_t u#a u#b a)
+      (t : ST.prog_tree a pre post) (sl0 : Fl.flist pre)
+  : Tot (prog_tree a post) (decreases t)
+  = match t with
+  | ST.Tequiv pre post0 p ->   
+          Tret U.unit' U.Unit' (const_post post0) (Fl.dlist_of_f (Fl.apply_pequiv p sl0))
+  | ST.Tframe a pre post frame f ->
+          let (sl0', sl_frame) = Fl.splitAt_ty pre frame sl0 in
+          Tbind a a _ _ (repr_SF_of_ST f sl0') (fun x sl1' ->
+          Tret a x (frame_post post frame) (Fl.dlist_of_f (Fl.append sl1' sl_frame)))
+  | ST.Tspec a pre post req ens ->
+          Tspec a post (req sl0) (ens sl0)
+  | ST.Tret a x post ->
+          Tret a x post (Fl.dlist_of_f sl0)
+  | ST.Tbind a b pre itm post f g ->
+          Tbind a b  _ _ (repr_SF_of_ST f sl0) (fun x sl1 -> repr_SF_of_ST (g x) sl1)
+  | ST.TbindP a b pre post wp f g ->
+          TbindP a b _ wp f (fun x -> repr_SF_of_ST (g x) sl0)
+
+let rec shape_SF_of_ST
+      (#pre_n #post_n : nat) (t : ST.shape_tree pre_n post_n)
+  : Tot (shape_tree post_n) (decreases t)
+  = match t with
+  | ST.Sequiv n _ ->
+          Sret true n
+  | ST.Sframe pre_n post_n frame_n s_f ->
+          Sbind _ _ (shape_SF_of_ST s_f) (Sret true (post_n + frame_n))
+  | ST.Sspec pre_n post_n ->
+          Sspec post_n
+  | ST.Sret smp_ret n ->
+          Sret smp_ret n
+  | ST.Sbind pre_n itm_n post_n s_f s_g ->
+          Sbind _ _ (shape_SF_of_ST s_f) (shape_SF_of_ST s_g)
+  | ST.SbindP pre_n post_n s_g ->
+          SbindP _ (shape_SF_of_ST s_g)
+
+
+(*** Soundness *)
+
+val repr_SF_of_ST_req
+      (#a : Type u#a) (#pre : ST.pre_t u#b) (#post : ST.post_t u#a u#b a)
+      (t : ST.prog_tree a pre post)
+      (sl0 : Fl.flist pre)
+  : Lemma (ST.tree_req t sl0 <==> tree_req (repr_SF_of_ST t sl0))
+
+val repr_SF_of_ST_ens
+      (#a : Type u#a) (#pre : ST.pre_t u#b) (#post : ST.post_t u#a u#b a)
+      (t : ST.prog_tree a pre post)
+      (sl0 : Fl.flist pre) (res : a) (sl1 : Fl.flist (post res))
+  : Lemma (ST.tree_ens t sl0 res sl1 <==> tree_ens (repr_SF_of_ST t sl0) res sl1)
+
+val repr_SF_of_ST_shape
+      (#a : Type u#a) (#pre : ST.pre_t u#b) (#post : ST.post_t u#a u#b a)
+      (t : ST.prog_tree a pre post)
+      (#post_n : nat) (s : ST.shape_tree (L.length pre) post_n)
+      (sl0 : Fl.flist pre)
+  : Lemma (requires ST.prog_has_shape t s)
+          (ensures  prog_has_shape (repr_SF_of_ST t sl0) (shape_SF_of_ST s))
